testdata/export/embed_hidden_def_comprehension.cue
@@ -1,0 +1,3 @@
+_#Mapper: {#data: [string]: string, mapped: {for k, v in #data {"\(k)": v}}}
+#S: {#data: [string]: string, _#Mapper}
+out: #S & {#data: {baz: "qux", foo: "bar"}}
