testdata/export/embed_hidden_def_sibling.cue
@@ -1,0 +1,3 @@
+_#Hidden: {#x: string, copy: #x}
+#S: {#x: string, _#Hidden}
+out: #S & {#x: "hi"}
