testdata/export/hidden_def_closed.cue
@@ -1,0 +1,2 @@
+_#Closed: {a: int}
+out: _#Closed & {a: 1}
